src/bijectionFin.lean
@@ -39,7 +39,9 @@ begin
   exact s1_fin,
 end
 
-lemma disjoint_union_preserves_fin (s1 s2: set A) [has_mem ↥(s1 ∪ s2) (set A)] [∀ (a:A) (s:set A), decidable (a ∈ s)] (s1_fin: is_finite s1) (s2_fin: is_finite s2) (disj: disjoint s1 s2): is_finite (s1 ∪ s2) :=
+def disjoint_union_bij (s1 s2: set A) (disj: disjoint s1 s2) {n1 n2: ℕ } (fs1: s1 → {x // x < n1}) (fs2: s2 → {x // x < n2}): (s1 ∪ s2) → {x // x < (n1 + n2)} := λ a, if a ∈ s1 then fs1 else n1 + fs2 
+
+lemma disjoint_union_preserves_fin (s1 s2: set A) [∀ (a:A) (s:set A), decidable (a ∈ s)] (s1_fin: is_finite s1) (s2_fin: is_finite s2) (disj: disjoint s1 s2): is_finite (s1 ∪ s2) :=
 begin
   unfold is_finite,
   unfold is_finite at s1_fin,
@@ -47,8 +49,26 @@ begin
   rcases s1_fin with ⟨n_s1, f_s1, f_s1_bij⟩,
   rcases s2_fin with ⟨n_s2, f_s2, f_s2_bij⟩,
   existsi (n_s1 + n_s2),
-  existsi ( λ (a: s1 ∪ s2), if a ∈ s1 then f_s1 a else f_s2 a),
+  existsi ( λ (a ∈  (s1 ∪ s2)), if a ∈ s1 then f_s1 a else (n_s1 + f_s2 a)),
   sorry,
+end
+
+lemma disjoint_union_preserves_fin (s1 s2: set A) [has_mem ↥(s1 ∪ s2) (set A)] [∀ (a:A) (s:set A), decidable (a ∈ s)] [has_mem ↥(s1 \ s2 ∪ s2) (set A)] [has_mem A (set A)] [∀ (a:A) (s:set A), decidable (a ∈ s)] (s1_fin: is_finite s1) (s2_fin: is_finite s2): is_finite (s1 ∪ s2) :=
+begin
+  by_cases int: s1 ∩ s2 = ∅,
+  apply disjoint_union_preserves_fin s1 s2 s1_fin s2_fin,
+  rw set.disjoint_iff_inter_eq_empty,
+  exact int,
+
+  have h: s1 ∪ s2 = (s1 \ s2) ∪ s2,
+  rw set.ext_iff,
+  intro x,
+  rw set.mem_union,
+  rw set.mem_union,
+  rw set.mem_diff,
+  tauto,
+  rw h,
+  apply disjoint_union_preserves_fin (s1 \ s2) s2,
 end
 
 end operations
